Simplified file. Regression in performance

rupicola/refinements2/CompilableWP.fst
@@ -11,16 +11,17 @@ let f () : Pure (nat -> nat) (z > 0) (fun _ -> True) by (dump "H") =
 (** Helpers to deal with Monotonicity of Pure **)
 module M = FStar.Monotonic.Pure
 
+  (**
 let intro_pure_wp_monotonicity (#a:Type) (wp:pure_wp' a)
   : Lemma
       (requires M.is_monotonic wp)
       (ensures pure_wp_monotonic a wp)
     [SMTPat (pure_wp_monotonic a wp)]
-  = M.intro_pure_wp_monotonicity wp
+  = M.intro_pure_wp_monotonicity wp **)
 
 unfold let (<=) #a (wp1 wp2:pure_wp a) = pure_stronger a wp1 wp2
 (** Using the ret is nicer, but makes things more fragile **)
-unfold let ret #a x : pure_wp a = fun p -> p x //pure_return a x //fun p -> p x
+unfold let ret #a x : pure_wp a = pure_return a x //fun p -> p x
 
 (** Typing environment **)
 type env = var -> option Type0
@@ -35,10 +36,11 @@ let extend (t:Type0) (g:env)
 (** F* evaluation environment **)
 assume val fs_env (g:env) : Type u#0
 assume val fs_empty : fs_env empty
-assume val get_v : #g:env -> fs_env g -> x:var{Some? (g x)} -> Some?.v (g x)
-assume val fs_extend : #g:env -> fsG:fs_env g -> #t:Type0 -> t -> fs_env (extend t g)
-assume val fs_shrink : #t:Type0 -> #g:env -> fs_env (extend t g) -> fs_env g
+assume val fs_top : #g:env{Some? (g 0)} -> fs_env g -> Some?.v (g 0)
+assume val fs_push : #g:env -> fsG:fs_env g -> #t:Type0 -> t -> fs_env (extend t g)
+assume val fs_pop : #t:Type0 -> #g:env -> fs_env (extend t g) -> fs_env g
 
+(**
 assume val lem_fs_extend #g (fsG:fs_env g) #t (v:t) : Lemma (
   (forall (x:var). Some? (g x) ==>  get_v fsG x == get_v (fs_extend fsG v) (x+1)) /\
   get_v (fs_extend fsG v) 0 == v)
@@ -48,8 +50,9 @@ assume val lem_fs_shrink #g #t (fsG:fs_env (extend t g)) : Lemma (
   (forall (x:var). Some? (g x) ==>  get_v fsG (x+1) == get_v (fs_shrink fsG) x))
   [SMTPat (fs_shrink fsG)]
 
-assume val shrink_extend_inverse #g (fsG:fs_env g) #t (x:t) : Lemma (fs_shrink (fs_extend fsG x) == fsG)
-  [SMTPat (fs_shrink (fs_extend fsG x))]
+assume val shrink_extend_inverse #g (fsG:fs_env g) #t (x:t) : Lemma (fs_pop (fs_push fsG x) == fsG)
+  [SMTPat (fs_pop (fs_push fsG x))]
+**)
 
 type spec_env (g:env) (a:Type) =
   fsG:fs_env g -> pure_wp a
@@ -59,31 +62,6 @@ type fs_oexp (g:env) (a:Type) (wpG:spec_env g a) =
   fsG:fs_env g -> PURE a (wpG fsG)
 
 unfold
-val wp_ref :
-  #g:env ->
-  #a:Type ->
-  ref1:(a -> Type0) ->
-  ref2:(a -> Type0) ->
-  wpV:spec_env g (x:a{ref1 x}) ->
-  spec_env g (x:a{ref2 x})
-let wp_ref #g #a ref1 ref2 wpV =
-  FStar.Monotonic.Pure.elim_pure_wp_monotonicity_forall ();
-  fun fsG (p:pure_post (x:a{ref2 x})) ->
-    wpV fsG (fun r -> ref2 r /\ p r)
-
-unfold
-val helper_ref : #g:env ->
-                 #a:Type ->
-                 #ref1:(a -> Type0) ->
-                 #ref2:(a -> Type0) ->
-                 #wpV:spec_env g (x:a{ref1 x}) ->
-                 v:fs_oexp g (x:a{ref1 x}) wpV ->
-                 fs_oexp g (x:a{ref2 x}) (wp_ref ref1 ref2 wpV)
-let helper_ref #g #a #ref1 #ref2 #wpV v =
-  FStar.Monotonic.Pure.elim_pure_wp_monotonicity_forall ();
-  fun fsG -> v fsG
-
-unfold
 val wp_lambda : #g :env ->
                 #a :Type ->
                 #b :Type ->
@@ -91,156 +69,49 @@ val wp_lambda : #g :env ->
                 spec_env g (a -> b)
 
 let wp_lambda #g #a #b wpBody fsG : pure_wp (a -> b) =
+  reveal_opaque (`%pure_wp_monotonic) pure_wp_monotonic;
   fun (p:pure_post (a -> b)) ->
     forall (f:a -> b).
       (forall (p':pure_post b) (fsG':fs_env (extend a g)).
-        fsG == fs_shrink fsG' ==>  wpBody fsG' p' ==>  p' (f (get_v fsG' 0))
+        fsG == fs_pop fsG' ==>  wpBody fsG' p' ==>  p' (f (fs_top fsG'))
       ) ==>  p f
-(**
- //  (forall f. p f) ==>
- //    (forall x. wpBody (fs_extend fsG x) (fun _ -> True)) /\
- //    (forall f. ret f p)
-
-
-  //  forall (fsG':fs_env (extend a g)). fsG == fs_shrink fsG' ==>
-  //    wpBody fsG' (fun r -> forall f. f fsG' (get_v fsG' 0) == r /\ p (f fsG'))
-**)
-
-unfold
-val helper_lambda : #g :env ->
-                    #a :Type ->
-                    #b :Type ->
-                    wpBody:spec_env (extend a g) b ->
-                    f :fs_oexp g (a -> b) (wp_lambda wpBody) ->
-                    fs_oexp (extend a g) b wpBody
-let helper_lambda #g #a #b wpBody f : fs_oexp (extend a g) b wpBody =
-  fun fsG -> f (fs_shrink #a fsG) (get_v fsG 0)
-
-unfold
-val helper_var : g:env ->
-                 a:Type ->
-                 x:var{Some? (g x) /\ a == Some?.v (g x)} ->
-                 fs_oexp g a (fun fsG p -> p (get_v fsG x))
-let helper_var g a x fsG = get_v fsG x
-
-unfold
-val helper_var1 : g:env ->
-                  a:Type ->
-                  b:Type ->
-                  x:var{Some? (g x) /\ a == Some?.v (g x)} ->
-                  fs_oexp (extend b g) a (fun fsG p -> p (get_v (fs_shrink #b fsG) x))
-let helper_var1 g a b x fsG = get_v (fs_shrink #b fsG) x
-
-unfold
-val helper_var2 : g:env ->
-                  a:Type ->
-                  b:Type ->
-                  c:Type ->
-                  x:var{Some? (g x) /\ a == Some?.v (g x)} ->
-                  fs_oexp (extend c (extend b g)) a (fun fsG p -> p (get_v (fs_shrink #b (fs_shrink #c fsG)) x))
-let helper_var2 g a b c x fsG = get_v (fs_shrink #b (fs_shrink #c fsG)) x
-
-unfold
-val fapp_wp : #g :env ->
-              #a :Type ->
-              #b :Type ->
-              wpF : spec_env g (a -> b) ->
-              wpX : spec_env g a ->
-              spec_env g b
-let fapp_wp #g #a #b wpF wpX fsG : pure_wp b =
-  FStar.Monotonic.Pure.elim_pure_wp_monotonicity_forall ();
-  fun (p:pure_post b) -> wpF fsG (fun f' -> wpX fsG (fun x' -> p (f' x')))
-
-unfold
-val helper_fapp : g :env ->
-                  a :Type ->
-                  b :Type ->
-                  wpF : spec_env g (a -> b) ->
-                  f :fs_oexp g (a -> b) wpF ->
-                  wpX : spec_env g a ->
-                  x :fs_oexp g a wpX ->
-                  fs_oexp g b (fapp_wp wpF wpX)
-
-let helper_fapp g a b wpF f wpX x : fs_oexp g b (fapp_wp wpF wpX) =
-  FStar.Monotonic.Pure.elim_pure_wp_monotonicity_forall ();
-  fun fsG -> (f fsG) (x fsG)
-
-unfold
-val if_wp : #g :env ->
-            #a :Type ->
-            wpC : spec_env g bool ->
-            wpT : spec_env g a ->
-            wpE : spec_env g a ->
-            spec_env g a
-let if_wp #g #a wpC wpT wpE fsG : pure_wp a =
-  FStar.Monotonic.Pure.elim_pure_wp_monotonicity_forall ();
-  fun (p:pure_post a) ->
-    wpC fsG (fun r -> (r == true ==> wpT fsG p) /\ (r == false ==> wpE fsG p))
-
-unfold
-val helper_if : #g :env ->
-                #a :Type ->
-                #wpC : spec_env g bool ->
-                c   : fs_oexp g bool wpC ->
-                #wpT : spec_env g a ->
-                t   : fs_oexp g a wpT ->
-                #wpE : spec_env g a ->
-                e   : fs_oexp g a wpE ->
-                fs_oexp g a (if_wp wpC wpT wpE)
-let helper_if c t e fsG =
-  FStar.Monotonic.Pure.elim_pure_wp_monotonicity_forall ();
-  if c fsG then t fsG else e fsG
-
-unfold
-val wp_seq :     #g:env ->
-                 ref1:Type0 ->
-                 wpV:spec_env g (x:unit{ref1}) ->
-                 #a:Type ->
-                 wpK:spec_env g a ->
-                 spec_env g a
-let wp_seq ref1 wpV wpK fsG =
-  FStar.Monotonic.Pure.elim_pure_wp_monotonicity_forall ();
-  fun p -> wpV fsG (fun _ -> wpK fsG p)
-
-unfold
-val helper_seq : #g:env ->
-                 ref1:Type0 ->
-                 #wpV:spec_env g (x:unit{ref1}) ->
-                 v:fs_oexp g (x:unit{ref1}) wpV -> (** since this is pure, I don't have to compile it **)
-
-                 #a:Type ->
-                 #wpK:spec_env g a ->
-                 k:fs_oexp g a wpK ->
-                 fs_oexp g a (wp_seq ref1 wpV wpK)
-let helper_seq ref1 v k =
-  FStar.Monotonic.Pure.elim_pure_wp_monotonicity_forall ();
-  fun fsG -> v fsG ; k fsG
 
 [@@no_auto_projectors] // FStarLang/FStar#3986
 noeq
 type compilable : #a:Type -> g:env -> wp:spec_env g a -> fs_oexp g a wp -> Type =
-| CUnit       : #g:env -> compilable g (fun _ p -> p ()) (fun _ -> ())
-| CTrue       : #g:env -> compilable g (fun _ p -> p true) (fun _ -> true)
-| CFalse      : #g:env -> compilable g (fun _ p -> p false) (fun _ -> false)
+| CUnit       : #g:env ->
+                compilable g
+                  (fun _ -> pure_return _ ())
+                  (fun _ -> ())
+| CTrue       : #g:env ->
+                compilable g
+                  (fun _ -> pure_return _ true)
+                  (fun _ -> true)
+| CFalse      : #g:env ->
+                compilable g
+                  (fun _ -> pure_return _ false)
+                  (fun _ -> false)
 
-(** The following three rules for variables should be generalized. What would be an elegant solution? **)
-| CVar0       : #g:env ->
-                #a:Type ->
-                #_:squash (Some? (g 0) /\ a == Some?.v (g 0)) ->
-                compilable #a g _ (helper_var g a 0)
-| CVar1       : #g:env ->
-                #a:Type ->
+(** Can we generalize the following three rules? **)
+| CVar0       : #g:env{Some? (g 0)} ->
+                #a:Type{a == Some?.v (g 0)} ->
+                compilable #a g
+                  (fun fsG -> pure_return _ (fs_top fsG))
+                  (fun fsG -> fs_top fsG)
+| CVar1       : #g:env{Some? (g 0)} ->
+                #a:Type{a == Some?.v (g 0)} ->
                 #b:Type ->
-                #_:squash (Some? (g 0) /\ a == Some?.v (g 0)) ->
- //               compilable #a (extend b g) (fun fsG p -> p (get_v fsG (x+1))) (fun fsG -> get_v fsG (x+1)) ->
-                compilable #a (extend b g) _ (helper_var1 g a b 0)
-| CVar2       : #g:env ->
-                #a:Type ->
+                compilable #a (extend b g)
+                  (fun fsG -> pure_return _ (fs_top (fs_pop #b fsG)))
+                  (fun fsG -> fs_top (fs_pop #b fsG))
+| CVar2       : #g:env{Some? (g 0)} ->
+                #a:Type{a == Some?.v (g 0)} ->
                 #b:Type ->
                 #c:Type ->
-                #_:squash (Some? (g 0) /\ a == Some?.v (g 0)) ->
- //               compilable #a (extend c (extend b g)) (fun fsG p -> p (get_v fsG (x+2))) (fun fsG -> get_v fsG (x+2)) ->
-                compilable #a (extend c (extend b g)) _ (helper_var2 g a b c 0)
+                compilable #a (extend c (extend b g))
+                  (fun fsG ->
+                    pure_return _ (fs_top (fs_pop #b (fs_pop #c fsG))))
+                  (fun fsG -> fs_top (fs_pop #b (fs_pop #c fsG)))
 
 | CApp        : #g :env ->
                 #a :Type ->
@@ -251,7 +122,13 @@ type compilable : #a:Type -> g:env -> wp:spec_env g a -> fs_oexp g a wp -> Type 
                 #wpX : spec_env g a ->
                 #x :fs_oexp g a wpX ->
                 cx:compilable g wpX x ->
-                compilable g _ (helper_fapp g a b wpF f wpX x)
+                compilable g
+                  (fun fsG ->
+                    pure_bind_wp _ _ (wpF fsG) (fun f' ->
+                      pure_bind_wp _ _ (wpX fsG) (fun x' ->
+                        pure_return _ (f' x'))))
+                  (fun fsG -> M.elim_pure_wp_monotonicity_forall ();
+                    (f fsG) (x fsG))
 
 | CIf         : #g :env ->
                 #a :Type ->
@@ -264,14 +141,22 @@ type compilable : #a:Type -> g:env -> wp:spec_env g a -> fs_oexp g a wp -> Type 
                 #wpE : spec_env g a ->
                 #e   : fs_oexp g a wpE ->
                 ce   : compilable g wpE e ->
-                compilable g _ (helper_if c t e)
+                compilable g
+                  (fun fsG ->
+                    pure_bind_wp _ _ (wpC fsG) (fun r ->
+                      pure_if_then_else _ r (wpT fsG) (wpE fsG)))
+                  (fun fsG ->
+                    M.elim_pure_wp_monotonicity_forall ();
+                    if c fsG then t fsG else e fsG)
 
 | CLambda     : #g :env ->
                 #a :Type ->
                 #b :Type ->
                 #wpBody:spec_env (extend a g) b ->
                 #f :fs_oexp g (a -> b) (wp_lambda wpBody) ->
-                cf:compilable #b (extend a g) wpBody (helper_lambda wpBody f) ->
+                cf:compilable #b (extend a g)
+                              wpBody
+                              (fun fsG -> f (fs_pop #a fsG) (fs_top fsG)) ->
                 compilable g _ f
 
 | CRefinement : #g:env ->
@@ -281,7 +166,19 @@ type compilable : #a:Type -> g:env -> wp:spec_env g a -> fs_oexp g a wp -> Type 
                 #wpV:spec_env g (x:a{ref1 x}) ->
                 #v:fs_oexp g (x:a{ref1 x}) wpV ->
                 compilable g wpV v ->
-                compilable g _ (helper_ref #g #a #ref1 #ref2 #wpV v)
+                compilable g
+                  (fun fsG ->
+                    pure_bind_wp (x:a{ref1 x}) (x:a{ref2 x}) (wpV fsG) (fun r ->
+                      M.as_pure_wp (fun (p:pure_post (x:a{ref2 x})) -> ref2 r /\ p r)))
+//                    pure_bind_wp _ _ (pure_assert_wp0 (ref2 r))
+//                      (fun _ -> pure_return (x:a{ref2 x}) r)))
+
+//                   M.elim_pure_wp_monotonicity_forall ();
+//                    M.as_pure_wp (fun (p:pure_post (x:a{ref2 x})) ->
+//                      wpV fsG (fun r -> ref2 r /\ p r)))
+                  (fun fsG ->
+                    M.elim_pure_wp_monotonicity_forall ();
+                    v fsG)
 
 | CSeq        : #g:env ->
                 ref1:Type0 ->
@@ -295,14 +192,19 @@ type compilable : #a:Type -> g:env -> wp:spec_env g a -> fs_oexp g a wp -> Type 
                 #wpK:spec_env g a ->
                 #k:fs_oexp g a wpK ->
                 compilable g wpK k ->
-                compilable g _ (helper_seq ref1 v k)
+                compilable g
+                  (fun fsG -> pure_bind_wp (x:unit{ref1}) a (wpV fsG) (fun _ -> wpK fsG))
+                  (fun fsG -> M.elim_pure_wp_monotonicity_forall ();
+                    v fsG ; k fsG)
 
+type compilable_closed #a #wp (x:a{forall fsG. wp fsG <= ret x}) =
+  compilable empty wp (fun _ -> x)
 
-unfold let compilable_closed #a #wp (x:a{forall fsG. wp fsG <= ret x}) =
+type compilable_debug #a wp (x:a{forall fsG. wp fsG <= ret x}) =
   compilable empty wp (fun _ -> x)
 
 let test2_var
-  : compilable (extend unit (extend unit empty)) _ (fun fsG -> get_v (fs_shrink fsG) 0)
+  : compilable (extend unit (extend unit empty)) _ (fun fsG -> fs_top (fs_pop fsG))
   = CVar1
 
 let test1_exp
@@ -331,7 +233,7 @@ let test1_comp_ref
 
 let test1_erase_ref
   : compilable_closed #(x:bool{x == true} -> bool) (fun x -> x)
-  = CLambda (CRefinement (fun x -> x == true) CVar0)
+  = CLambda (CRefinement (fun x -> x == true) #(fun _ -> True) CVar0)
 
 open Examples
 
@@ -372,20 +274,6 @@ let test_if_x'
   : compilable_closed test_if_x
   = CLambda (CLambda (CIf CVar0 (CApp CVar1 (CRefinement (fun _ -> True) #(fun x -> x == true) CVar0)) CFalse))
 
-let test_p_implies_q'
-  : compilable_closed test_p_implies_q
-  = CLambda (CLambda (CSeq q_ref (CApp CVar1 CVar0) (CRefinement p_ref #(fun _ -> q_ref) CVar0)))
- // = CLambda (CLambda (CApp (CLambda (CRefinement p_ref #(fun _ -> q_ref) CVar1)) (CApp CVar1 CVar0)))
-
-let test_true_implies_q
-  : compilable_closed test_true_implies_q
-  = CLambda (CLambda (
-     CIf CVar0
-         (CSeq q_ref (CApp CVar1 (CRefinement (fun _ -> True) #(fun x -> x == true) CVar0))
-                     (CRefinement (fun _ -> True) #(fun x -> x == true ==> q_ref) CVar0))
-         (CRefinement (fun _ -> True) #(fun x -> x == true ==> q_ref) CFalse)))
-
-
 let test_context
   : (x:bool) -> (f:(x:bool{x == true}) -> bool -> bool) -> bool -> bool
   = fun x f ->
@@ -398,3 +286,16 @@ let test_context'
   = CLambda (CLambda (CIf CVar1
                           (CApp CVar0 (CRefinement (fun _ -> True) #(fun x -> x == true) CVar1))
                           (CLambda #_ #_ #_ #_ #(fun fsG y -> y) CVar0)))
+
+let test_p_implies_q'
+  : compilable_debug _ test_p_implies_q
+  = CLambda (CLambda (CSeq q_ref (CApp CVar1 CVar0) (CRefinement p_ref CVar0)))
+ // = CLambda (CLambda (CApp (CLambda (CRefinement p_ref #(fun _ -> q_ref) CVar1)) (CApp CVar1 CVar0)))
+
+let test_true_implies_q
+  : compilable_closed _ test_true_implies_q
+  = CLambda (CLambda (
+     CIf CVar0
+         (CSeq q_ref (CApp CVar1 (CRefinement (fun _ -> True) #(fun x -> x == true) CVar0))
+                     (CRefinement (fun _ -> True) #(fun x -> x == true ==> q_ref) CVar0))
+         (CRefinement (fun _ -> True) #(fun x -> x == true ==> q_ref) CFalse)))
